Phi_Semantics/PhiSem_Common_Int.thy
@@ -151,10 +151,10 @@ lemma synthesis_const:
 *)
 
 lemma synthesis_const_by_imp:
-  \<open> R \<t>\<r>\<a>\<n>\<s>\<f>\<o>\<r>\<m>\<s> const \<Ztypecolon> \<v>\<a>\<l>[\<phi>literal v] T \<r>\<e>\<m>\<a>\<i>\<n>\<s> R @action synthesis
-\<Longrightarrow> \<p>\<r>\<o>\<c> Return (\<phi>literal v) \<lbrace> R \<longmapsto> \<lambda>ret. const \<Ztypecolon> \<v>\<a>\<l>[ret] T \<r>\<e>\<m>\<a>\<i>\<n>\<s> R \<rbrace> @action synthesis\<close>
+  \<open> R \<t>\<r>\<a>\<n>\<s>\<f>\<o>\<r>\<m>\<s> const \<Ztypecolon> \<v>\<a>\<l>[\<phi>literal v] T \<r>\<e>\<m>\<a>\<i>\<n>\<s> R' @action synthesis
+\<Longrightarrow> \<p>\<r>\<o>\<c> Return (\<phi>literal v) \<lbrace> R \<longmapsto> \<lambda>ret. const \<Ztypecolon> \<v>\<a>\<l>[ret] T \<r>\<e>\<m>\<a>\<i>\<n>\<s> R' \<rbrace> @action synthesis\<close>
   unfolding Action_Tag_def Premise_def \<phi>Procedure_def det_lift_def Return_def \<phi>literal_def Transformation_def
-  by (clarsimp simp add: Val.unfold INTERP_SPEC_subj Subjection_expn_set INTERP_SPEC)
+  by (clarsimp simp add: Val.unfold INTERP_SPEC_subj Subjection_expn_set INTERP_SPEC, blast)
 
 
 (*lemma make_synthesis_rule_for_const:
