Phi_Semantics/PhiSem_Machine_Integer.thy
@@ -528,7 +528,8 @@ subsubsection \<open>Constant Integer\<close>
 
 lemma op_const_word_\<phi>app[\<phi>reason %ToA_mk_literal_cut]:
   \<open> \<s>\<i>\<m>\<p>\<l>\<i>\<f>\<y>[\<phi>mode_literal] n : unat n'
-\<Longrightarrow> X \<t>\<r>\<a>\<n>\<s>\<f>\<o>\<r>\<m>\<s> X \<heavy_comma> n' \<Ztypecolon> \<v>\<a>\<l>[\<phi>literal (V_int.mk (LENGTH('b),n))] Word('b)\<close>
+\<Longrightarrow> X \<t>\<r>\<a>\<n>\<s>\<f>\<o>\<r>\<m>\<s> n' \<Ztypecolon> \<v>\<a>\<l>[\<phi>literal (V_int.mk (LENGTH('b),n))] Word('b) \<r>\<e>\<m>\<a>\<i>\<n>\<s> X @action synthesis\<close>
+  for X :: assn
 \<medium_left_bracket>
   semantic_literal \<open>V_int.mk (LENGTH('b),n) \<Turnstile> (n' \<Ztypecolon> Word('b))\<close>
 \<medium_right_bracket> .
@@ -536,7 +537,8 @@ lemma op_const_word_\<phi>app[\<phi>reason %ToA_mk_literal_cut]:
 lemma op_const_nat_\<phi>app[\<phi>reason %ToA_mk_literal_cut]:
   \<open> \<p>\<r>\<e>\<m>\<i>\<s>\<e> n < 2 ^ LENGTH('b)
 \<Longrightarrow> \<s>\<i>\<m>\<p>\<l>\<i>\<f>\<y>[\<phi>mode_literal] n' : n
-\<Longrightarrow> X \<t>\<r>\<a>\<n>\<s>\<f>\<o>\<r>\<m>\<s> X \<heavy_comma> n \<Ztypecolon> \<v>\<a>\<l>[\<phi>literal (V_int.mk (LENGTH('b),n'))] \<nat>('b)\<close>
+\<Longrightarrow> X \<t>\<r>\<a>\<n>\<s>\<f>\<o>\<r>\<m>\<s> n \<Ztypecolon> \<v>\<a>\<l>[\<phi>literal (V_int.mk (LENGTH('b),n'))] \<nat>('b) \<r>\<e>\<m>\<a>\<i>\<n>\<s> X @action synthesis\<close>
+  for X :: assn
 \<medium_left_bracket>
   semantic_literal \<open>V_int.mk (LENGTH('b),n') \<Turnstile> (n \<Ztypecolon> \<nat>('b))\<close>
   certified by (simp add: \<phi> unat_of_nat_len)
@@ -546,7 +548,8 @@ declare [[\<phi>trace_reasoning = 2]]
 
 lemma op_const_natR_\<phi>app[\<phi>reason %ToA_mk_literal_cut]:
   \<open> \<s>\<i>\<m>\<p>\<l>\<i>\<f>\<y>[\<phi>mode_literal] n' : n mod 2 ^ LENGTH('b)
-\<Longrightarrow> X \<t>\<r>\<a>\<n>\<s>\<f>\<o>\<r>\<m>\<s> X \<heavy_comma> n \<Ztypecolon> \<v>\<a>\<l>[\<phi>literal (V_int.mk (LENGTH('b),n'))] \<nat>\<^sup>r('b)\<close>
+\<Longrightarrow> X \<t>\<r>\<a>\<n>\<s>\<f>\<o>\<r>\<m>\<s> n \<Ztypecolon> \<v>\<a>\<l>[\<phi>literal (V_int.mk (LENGTH('b),n'))] \<nat>\<^sup>r('b) \<r>\<e>\<m>\<a>\<i>\<n>\<s> X @action synthesis\<close>
+  for X :: assn
 \<medium_left_bracket>
   apply_rule op_const_word[where 'b='b and n=n' and n' = \<open>of_nat n\<close>, simplified, OF Simplify_to_Premise]
   certified by (simp add: the_\<phi>(2) unat_of_nat) 
